Use new function syntax

Test/ast/function.dfy
@@ -1,13 +1,13 @@
-// RUN: %baredafny verify --use-basename-for-filename "%s" > "%t"
-// RUN: ! %baredafny run --use-basename-for-filename "%s" >> "%t"
+// RUN: %baredafny verify --function-syntax:4 --use-basename-for-filename "%s" > "%t"
+// RUN: ! %baredafny run --function-syntax:4 --use-basename-for-filename "%s" >> "%t"
 // RUN: %diff "%s.expect" "%t"
 
-function method Foo(): int ensures false; ensures false;
-function method {:axiom} Bar(): int ensures false;
-function method {:extern} Baz(): int ensures false;
-function method Fonk(): int ensures {:axiom} false;
-function method Faz(): int
+function Foo(): int ensures false; ensures false;
+function {:axiom} Bar(): int ensures false;
+function {:extern} Baz(): int ensures false;
+function Fonk(): int ensures {:axiom} false;
+function Faz(): int
 
 trait Far {
-  function method Foo(): int
+  function Foo(): int
 }
